src/Enumerators.v
@@ -15,57 +15,7 @@ Import MonadNotation.
 Open Scope monad_scope.
 
 From QuickChick Require Import
-     Sets Tactics Producer LazyList.
-
-Set Implicit Arguments.
-Unset Strict Implicit.
-Unset Printing Implicit Defensive.
-
-Set Bullet Behavior "Strict Subproofs".
-
-Import ListNotations.
-
-(* Low-level Generators *)
-
-Open Scope fun_scope.
-Open Scope set_scope.
-
-Inductive EnumType (A:Type) : Type :=
-  MkGen : (nat -> LazyList A) -> EnumType A.
-  
-Definition E := EnumType.
-
-(** * Primitive generator combinators *)
-
-Definition run {A : Type} (g : E A) :=
-  match g with MkGen f => f end.
-
-Definition returnEnum {A : Type} (x : A) : E A :=
-  MkGen (fun _ => ret x).
-
-  
-Definition bindEnum {A B : Type} (g : E A) (k : A -> E B) : E B :=
-  MkGen (fun n =>
-           x <- run g n;;
-           run (k x) n).
-
-Instance MonadEnum : Monad E :=
-  { ret := @returnEnum
-  ; bind := @bindEnum }.
-
-Definition sampleEnum (A : Type) (g : E A) : list A :=
-  LazyList_to_list (run g 4).
-
-Definition sizedEnum {A : Type} (f : nat -> E A) : E A :=
-  MkGen (fun n => run (f n) n).
-
-Definition resizeEnum {A : Type} (n : nat) (g : E A) : E A :=
-    match g with
-    | MkGen m => MkGen (fun _ => m n)
-    end.
-
-Definition semEnumSize {A : Type} (g : E A) (s : nat) : set A :=
-  fun x => In_ll x (run g s).
+     Sets Tactics Producer LazyList RandomQC.
 
 Program Instance ProducerEnum : Producer E :=
   {
@@ -76,6 +26,8 @@ Program Instance ProducerEnum : Producer E :=
   sized  := @sizedEnum; 
   resize := @resizeEnum;
 
+  choose := @chooseEnum;
+  
   semProdSize := @semEnumSize;
 
   (* Probably belongs in another class for modularity? *)
@@ -101,5 +53,3 @@ Next Obligation.
   apply (X n).
 Defined.
 
-Print ProducerEnum.
-Print ProducerEnum_obligation_1.
